SimplePCFa: add type env strengthening lemma

proof/DDC/Language/SimplePCFa/TyJudge.v
@@ -1,32 +1,35 @@
 
+Require Export DDC.Language.SimplePCFa.ExpLower.
+Require Export DDC.Language.SimplePCFa.ExpRefs.
 Require Export DDC.Language.SimplePCFa.Exp.
 Require Export DDC.Language.SimplePCFa.Ty.
 
 
-Inductive TYPEX : tyenv -> exp -> ty -> Prop :=
- | TxVar
+Inductive TYPEV : tyenv -> val -> ty -> Prop := 
+ | TvVar
    :  forall te i t
    ,  get i te = Some t
-   -> TYPEX te (XVal (VVar i)) t
+   -> TYPEV te (VVar i) t
 
- | TxConstBool
+ | TvConstBool
    :  forall te b
-   ,  TYPEX te (XVal (VConst (CBool b))) tBool
+   ,  TYPEV te (VConst (CBool b)) tBool
 
- | TxConstNat
+ | TvConstNat
    :  forall te n
-   ,  TYPEX te (XVal (VConst (CNat n))) tNat
+   ,  TYPEV te (VConst (CNat n)) tNat
 
- | TxLam
+ | TvFix
+   :  forall te t1 v2
+   ,  TYPEV (te :> t1) v2 t1
+   -> TYPEV te (VFix t1 v2) t1
+
+ | TvLam
    :  forall te t1 t2 x2
    ,  TYPEX (te :> t1) x2 t2
-   -> TYPEX te (XVal (VLam t1 x2)) (TFun t1 t2)
+   -> TYPEV te (VLam t1 x2) (TFun t1 t2)
 
- | TxFix
-   :  forall te t1 v2
-   ,  TYPEX (te :> t1) (XVal v2) t1
-   -> TYPEX te (XVal (VFix t1 v2)) t1
-
+ with TYPEX : tyenv -> exp -> ty -> Prop :=
  | TxLet
    :  forall te t1 x1 t2 x2
    ,  TYPEX (te :> t1) x2 t2
@@ -34,30 +37,74 @@ Inductive TYPEX : tyenv -> exp -> ty -> Prop :=
 
  | TxApp
    :  forall te t11 t12 v1 v2
-   ,  TYPEX te (XVal v1) (TFun t11 t12) 
-   -> TYPEX te (XVal v2) t11
+   ,  TYPEV te v1 (TFun t11 t12) 
+   -> TYPEV te v2 t11
    -> TYPEX te (XApp v1 v2) t12
 
  | TxOpSucc
    :  forall te v1
-   ,  TYPEX te (XVal v1) tNat
+   ,  TYPEV te v1 tNat
    -> TYPEX te (XOp1 OSucc v1) tNat
 
  | TxOpPred
    :  forall te v1
-   ,  TYPEX te (XVal v1) tNat
+   ,  TYPEV te v1 tNat
    -> TYPEX te (XOp1 OPred v1) tNat
 
  | TxOpIsZero
    :  forall te v1
-   ,  TYPEX te (XVal v1) tNat
+   ,  TYPEV te v1 tNat
    -> TYPEX te (XOp1 OIsZero v1) tBool
 
  | TxIf
    :  forall te v1 x2 x3 tR
-   ,  TYPEX te (XVal v1) tBool
+   ,  TYPEV te v1 tBool
    -> TYPEX te x2 tR
    -> TYPEX te x3 tR
    -> TYPEX te (XIf v1 x2 x3) tR.
+Hint Constructors TYPEV.
 Hint Constructors TYPEX.
+
+
+Lemma type_tyenv_delete
+ :  forall te x t ix
+ ,  ~(refsXX ix x)
+ -> TYPEX te x t 
+ -> TYPEX (delete ix te) (lowerXX ix x) t.
+Proof.
+ intros. gen te t ix.
+ induction x using exp_mutind with 
+  (PV := fun v => forall te t ix
+      ,  ~(refsXV ix v)
+      -> TYPEV te v t
+      -> TYPEV (delete ix te) (lowerXV ix v) t);
+ intros; inverts H0; simpl; eauto.
+
+ Case "VVar".
+  destruct n.
+   eapply TvVar. admit. (* ok list lemma *)
+   lift_cases. 
+    eapply TvVar. admit. (* ok list lemma *)
+    eapply TvVar. eauto.
+
+ Case "VLam".
+  eapply TvLam. simpl in H.
+  rewrite delete_rewind. eauto.
+
+ Case "VFix".
+  eapply TvFix. simpl in H.
+  rewrite delete_rewind. eauto.
+
+ Case "XLet".
+  eapply TxLet. simpl in H.
+  rewrite delete_rewind. eauto.
+
+ Case "XApp".
+  simpl in H.
+  eapply TxApp; burn.
+
+ Case "XIf".
+  simpl in H.
+  eapply TxIf; burn.
+Qed.
 
